#operations/factorising-and-expanding
**Links**
- [[Quadratics - Factorising examples]] 
#### Expanding
$a(b+c) = ab+ac$

$(a+b)(c+d) = ac +ad + bc +bd$

$(x+a)^{2} = x^{2} + 2ax + a^{2}$

$(x-a)^{2} = x^{2} - 2ax + a^{2}$

$(x-a)(x+a) = x^{2} - ax + ax - a^{2} = x^{2} - a^{2}$

#### Factorising
1. Identify a common factor ()
2. Express the expression as $c(E)$ where $E$ is the original expression divided by common factor $c$, like $3x^{2} +6x \rightarrow 3x(x+2)$


Factorising quadratics:
$(x+m)(x+n)$; $x^{2} + bx + c$
1. Check what values of $m$ and $n$ $=c$,  $m \times n = c$
2. Check what values of $m$ and $n$ $=c$,  $m + n = b$
3. Is there an $m$ and $n$ value that satisfies both equations?


$x^{2} - 4x - 5$
-> To get $5$, we need to times the numbers either by:
	- $-5$ and $+1$ or
	- $+5$ and $-1$
The correct one is the one that adds up to the $bx$ term,
	$-5 + 1 = -4x$
	$+5 - 1 = 4x$
So, the first term is correct.
From this, we can construct the factored result:
	$(x-5)(x+1)$


$x^{2} + x + \frac{1}{4} = (x+ \frac{1}{2})^{2}$
