---
tags:
  - portfolio/worksheets/3/2D
received-week: 3
due-week: 4
due-date: 2024-03-17
finished: true
submitted: true
todo: All
topics:
  - "[[Matrices]]"
  - "[[Polynomial functions]]"
---

### Task 1: Matrices - Inverses
\1) 
$$
\begin{bmatrix}  8 & -16  \\  -2 & 4  \end{bmatrix}
$$
**Determinant:** 
$\frac{1}{ad-bc}$
-> $8\times4 - -16\times-2$
-> $32 - 32 = 0$
Since $\frac{1}{0} = \text{undefined}$, this matrix does not have an inverse


\2)
$$
\begin{bmatrix}  5 & 2  \\  7 & 4  \end{bmatrix}
$$
**Determinant:** 
-> $5\times4 - 2\times7$
-> $20 - 14 = 6$
-> $\frac{1}{6}$
The determinant is non-zero, so the matrix does have an inverse

**Inverse:**
$$
\begin{bmatrix}  5 & 2  \\  7 & 4  \end{bmatrix} \rightarrow \begin{bmatrix}  4 & -2  \\  -7 & 5  \end{bmatrix} \times \frac{1}{6} =\begin{bmatrix}\frac{2}{3} & -\frac{1}{3} \cr -\frac{7}{6} & \frac{5}{6}\end{bmatrix}
$$

### Task 2: Simultaneous equations
Sakae bought 4 pens, 2 notepads, and paid \$13
Pritika bough 8 pens, 1 notepads, and paid \$8

*What was the cost/pen and cost/notebook?*

$$
\left \{
    \begin{array}{l}
	4p + 2n = 13  &\\
	8p + 1n = 8  &\\
 \end{array}
\right.
$$
$$
\begin{bmatrix} 4 & 2 \\ 8 & 1 \end{bmatrix}
\begin{bmatrix} p \\ n \end{bmatrix}
= \begin{bmatrix} 13 \\ 8 \end{bmatrix}
$$

Determinant: $ad-bc$
$4\times1 - 2\times8 = -12$
There therefore is a valid inverse matrix. We will times the flipped matrix using $\frac{1}{-12}$.
$$
\begin{bmatrix}  4 & 2  \\  8 & 1  \end{bmatrix} 
\rightarrow
\begin{bmatrix}  1 & -2  \\  -8 & 4  \end{bmatrix}
$$
$$
-\frac{1}{12} \times \begin{bmatrix}  1 & -2  \\  -8 & 4  \end{bmatrix}
=
\begin{bmatrix}  
   -\frac{1}{12} & \frac{2}{12}  \\
   \frac{8}{12} & - \frac{4}{12}
\end{bmatrix}
=
\begin{bmatrix}
    - \frac{1}{12} & \frac{1}{6} \\ 
    \frac{2}{3} & - \frac{1}{3}
\end{bmatrix}
$$

Now that we have the inverse matrix, we can multiply both sides of the equation by it, removing the non-inverted matrix and finding the solution for the $\begin{bmatrix}  p  \\  n \end{bmatrix}$ matrix.

Full equation:
$$
\begin{bmatrix}
    - \frac{1}{12} & \frac{1}{6} \\ 
    \frac{2}{3} & - \frac{1}{3}
\end{bmatrix}

\begin{bmatrix} 4 & 2 \\ 8 & 1 \end{bmatrix}
\begin{bmatrix} p \\ n \end{bmatrix}
= 
\begin{bmatrix}
    - \frac{1}{12} & \frac{1}{6} \\ 
    \frac{2}{3} & - \frac{1}{3}
\end{bmatrix}

\begin{bmatrix} 13 \\ 8 \end{bmatrix}
$$

Solving $A \times A^{-1}$ 
$$
\begin{bmatrix}  
    - \frac{1}{12}\times4 + \frac{1}{6}\times8 &  - \frac{1}{12} \times 2 + \frac{1}{6}\times 1\\  
    \frac{2}{3}\times4 + -\frac{1}{3}\times8 &
    \frac{2}{3}\times2 + -\frac{1}{3}\times1
\end{bmatrix}
\rightarrow
\begin{bmatrix}  1 & 0  \\  0 & 1  \end{bmatrix}
$$
$$
\begin{bmatrix}  1 & 0  \\  0 & 1  \end{bmatrix}
\begin{bmatrix}  p  \\  n  \end{bmatrix}
=
\begin{bmatrix}
    1\times p + 0 \times n \\
    0 \times p + 1 \times n 
\end{bmatrix}
=
\begin{bmatrix}  p  \\  n  \end{bmatrix}
$$

Solving $A^{-1} \times \begin{bmatrix}  13  \\  8  \end{bmatrix}$
$$
\begin{bmatrix}
    - \frac{1}{12} & \frac{1}{6} \\ 
    \frac{2}{3} & - \frac{1}{3}
\end{bmatrix}
\begin{bmatrix}  13  \\  8  \end{bmatrix}
=
\begin{bmatrix}
    -\frac{1}{12}\times13+\frac{1}{6}\times8 \\ 
    \frac{2}{3}\times13 + - \frac{1}{3}\times8
\end{bmatrix}
=
\begin{bmatrix}  - \frac{13}{12} + \frac{8}{6}  \\  \frac{26}{3} + - \frac{8}{3}  \end{bmatrix}
$$
$$
\begin{bmatrix}  - \frac{13}{12} + \frac{8}{6}  \\  \frac{26}{3} + - \frac{8}{3}  \end{bmatrix}
=
\begin{bmatrix}  - \frac{13}{12} + \frac{16}{12}=\frac{3}{12}  \\  \frac{18}{3}  \end{bmatrix}

=
\begin{bmatrix}  \frac{1}{4} \\ 6  \end{bmatrix}
$$

The matrix method is significantly quicker to do only if you have a calculator to quickly multiply matrices and find the inverse. Without a calculator, the elimination method seems to be best for me. Doing them manually and typing formulas for each answer was excruciating, without typing the working out and with a calculator, it is lightning fast. Matrices do not come intuitively to me, but it is ultimately very satisfying to see the answer 'appear' of nowhere.


### Task 3: Quadratics
Given $y=-x^{2}-3x-9$:

***Find the $x$ and $y$-intercepts***
-> $y=-0^{2} - 3(0) - 9$
	-> $= 0 - 0 - 9$
	-> $y=-9$

*x-intercept (method 1/3)*
-> $0 = -x^{2} - 3x - 9$
$x= \frac{ -b \pm \sqrt{ b^{2} - 4ac } }{ 2a }$ 
-> $\frac{ --3 \pm \sqrt{ -3^{2} - 4(-1)(-9) } }{ 2(-1) } = \frac{ 3 \pm \sqrt{ -27 }}{ -2 }$
-> $x^{+} = \frac{ 3 + \sqrt{ -27 }}{ -2 }$
-> $x^{-} = \frac{ 3 - \sqrt{ -27 }}{ -2 }$
There is no real x-intercept. It therefore must be below the x-axis.

*x-intercept (determinant method, 2/3)*
$0 = -x^{2} - 3x - 9$
Find the determinant: $\sqrt{b^{2} - 4ac}$
-> $-3^{2} - 4(-1)(-9)$
-> $9 - 4 \times 9 \rightarrow 9 - 36$
-> $\sqrt{-27}$
Since the determinant is $<0$, there are no real solutions.

*x-intercept algebraic method (3/3)*
Please don't use this answer as the solution for the x-intercept. The maths appears to check out to me but I clearly have done something wrong... could I have it explained why this is wrong?
-> $0 = -x^{2} - 3x - 9$
	-> $9 = -x^{2}-3x$
	-> $9+3x = -x^{2}$
	-> $12 = -\frac{x^{2}}{x}$
	-> $12 = -x$
	-> $x=-12$

-> $9+3x = -x^{2}$
-> $\frac{9+3x}{x} = \frac{-x^{2}}{x}$
-> $\frac{9}{x} + 3 = -x$
-> $12 = -x^{2}$
$x = \sqrt{-12}$


***Stationary point***
Formula given $y=ax^{2}+bx+c$
We want to reach the turning point formula format, $a(x-h)^{2}+k$

$-x^{2} - 3x - 9$
-> $+ \frac{b}{2}^{2}$ and $- \frac{b}{2}^{2}$ to both sides
	-> $\pm \frac{9}{4}$
-> $-x^{2}-3x + \frac{9}{4} -9 - \frac{9}{4}$
-> $(-x^{2} - 3x + \frac{3}{2}^{2}) - (9 - \frac{9}{4})$
	-> $(x+m)(x+n)$
	-> $m \times n = \frac{3}{2}^{2}: [(\frac{3}{2}, 1), (\frac{1}{2}, 3)]$
	-> $m + n = \frac{3}{2} + \frac{3}{2} = \frac{6}{2} = 3$
-> $y = -(x+ \frac{3}{2})^{2} - \frac{27}{4}$

From this, we know that we can translate the graph $- \frac{27}{4}$ down the $y$ coordinate and by $\frac{3}{2}$ across the $x$ coordinate. And remembering the translating by a positive number on the $x$ axis moves left instead of the intuitive right, this reaches the vertex of $(- \frac{3}{2}, - \frac{27}{4})$, or $(-1.5, -6.75)$

**Verification**
Using the vertex formula, $x = \ce{\frac{-b}{2a} -> \frac{--3}{2(-1)} -> -\frac{3}{2}}$
At this point, the vertex is equal to $(\frac{-3}{2}, y)$

We substitute $x$ into the found turning point formula to find the $y$ coordinate like so:
-> $y = -(\frac{-3}{2} + \frac{3}{2})^{2} - \frac{27}{4}$
-> $-(0)^{2} - \frac{27}{4}$
-> $y = \frac{-27}{4} = -6.75$
The vertex/stationary point is still $(-1.5, -6.75)$ 

**Graph**
The graph displays the vertex as a local (and global) maximum, being the highest point of the parabola

![[3.2D - Task 3 - Quadratics.jpg|200]]

### Task 4: Cubic
***Find the $x$ and $y$-intercepts of the cubic equation* $y=(x-3)(x^{2}-14)$**

$0 = x-3$
-> $x = 3$
$0 = x^{2} - 14$
-> $x = \pm \sqrt{14}$
The x intercepts are therefore:
$(3, 0), (\sqrt{14}, 0), (-\sqrt{14}, 0)$

*y-intercept*
$y = (0-3)(0^{2} - 14)$
-> $-3 \times - 14$
-> $y = 42$


**Verification**
![[3.2D - Task 4 cubic verification.png|200]]