**Links**
- [[Calculus]] 
- [[The Derivative]] 

$\frac{y_{2}-y_{1}}{x_{2}-x_{1}} = \frac{ f(x_{2}) - f(x_{1}) }{ x_{2} - x_{1} }$
= $\frac{ f(x_{1} + h) - f(x_{1}) }{ x_{1} + h - x_{1} }$
= $\frac{ f(x_{1} + h) - f(x_{1}) }{ h  }$


"As $h$ reaches a limit of $0$" or "as $h$ approaches $0$" 
$\lim_{h\to0} = \frac{ f(x_{1} + h) - f(x_{1}) }{ h  }$

The smaller the distance between $h$ and $0$, the closer the average rate of change is to the instantaneous rate of change of $f$ when $x=x_{1}$

#### When $h = 0$,
$\frac{ f(x_{1} + h) - f(x_{1}) }{ h  } = \frac{ f(x_{1}) - f(x_{1}) }{ h  } = \frac{0}{0}$


![[Rate of change - f(x) on top and x on bottom. Time (s) vs distance (m).png]]


