**Links**
- [[Logarithms (log)]] 
	- [[Log questions - Misc.]] 
- [[Log Laws - Addition]] 
- [[Log Laws - Subtraction]]
- [[Log Laws - Log(m raised to n)]]
- -\> [[Log Laws - Log base of base]]
	- [[Log questions - Log base of base]]
- [[Log Laws - Log of 1]]
- [[Log Laws - Changing logs]]

$log_{a}(a)=1$

$log_{b}(x)=y$
-> $b^{log_{b}(x)}=b^{y}$ 
Result: $x=b^{y}$

#### Examples
$log_{e}(e) = 1$
Think of it like "the amount of time for the growth to increase by $e$ is $e$"

##### $y=log_{5}(-5x+13)$, where $y=3$
$3=log_{5}(-5x+13)$
We want to remove the $log_{5}$, so we take the base ($5$) and then raise that to the log: $b^{y}$
-> $5^{3}=5^{log_{5}(-5x+13)}$
-> $125=-5x+13$
-> $112 = -5x$
-> $x=\frac{112}{-5}$
$x=-22.4$