---
tags:
  - portfolio/worksheets/9/1P
received-week: 10
due-week: 11
due-date: 2024-05-13T00:00:00
finished: true
submitted: true
todo: Give it a goes
topics:
  - "[[The Derivative]]"
---
# Task 1: Give it a go
![[9.1P - Give it a go 1.png|200]] ![[9.1P - Give it a go again.png|200]]

For nearly every question, there were indefinite integrals that required a $C$ constant to be placed at the end. I forgot every single time. I need to work on remembering this important step. I understand how to solve for $C$ which is excellent.
In the first attempt, I struggled to understand why fractions like $\frac{1}{x^{3}}$ becomes $- \frac{1}{2x^{2}}$ instead of $- \frac{2}{x^{2}}$, and I still do struggle to understand to some degree but it is slowly sinking in. 
Another bonus is that I am beginning to be able to calculate this stuff all mentally with no writing down. With this new power though, I am repeating silly mistakes all over again but that seems to be the case with any sort of new skill.

I will focus on mental calculations more to hone the skill further as it is extremely gratifying and also speeds up calculations significantly.


# Task 2: Anti-differentiation
### 1) Integrate the following functions
##### a) Integrate $\int (5x^{4} - 27x^{3} + 38x^{2})$
$\int (5x^{4} - 27x^{3} + 38x^{2}) + C$
-> $\frac{5x^{4+1}}{4+1}  -  \frac{27x^{3+1}}{3+1} + \frac{38x^{2+1}}{2+1} + C$
-> $\frac{5x^{5}}{5}  -  \frac{27x^{4}}{4} + \frac{38x^{3}}{3} + C$
-> $\frac{5}{5}x^{5}  -  \frac{27}{4}x^{4} + \frac{38}{3}x^{3} + C$
$= x^{5}  -  \frac{27}{4}x^{4} + \frac{38}{3}x^{3} + C$


##### b) Integrate $\int ( \frac{13}{x^{3}} - \frac{26}{x} + 10x^{\frac{17}{23}} )$
$\int \left( \frac{13}{x^{3}} - \frac{26}{x} + 10x^{\frac{17}{23}} \right)+ C$
When written in power notation, $\frac{26}{x}$ becomes $26x^{-1}$. If we then find the integral of this, it becomes $\frac{26x^{0}}{0}$. A division by $0$ is not allowed, so we instead convert it to the log version where $\ln(u)' = \frac{1}{u}$ and then reverse it.
We apply the $|x|$ absolute function to the $x$ as in log functions, it can not be $\leq 0$.
-> $13x^{-3} - 26\ln(|x|) + 10x^{\frac{17}{23}}+ C$
-> $\frac{13x^{-3+1}}{-3+1} - 26\ln(|x|) + \frac{ 10x^{\frac{17}{23} + \frac{23}{23} }  }{ \frac{17}{23} + \frac{23}{23} } + C$
-> $\frac{13x^{-2}}{-2} - 26\ln(|x|) + \frac{ 10x^{\frac{40}{23} }  }{ \frac{40}{23} } + C$
-> $- \frac{13}{2}x^{-2} - 26\ln(|x|) + \frac{23}{4}x^{\frac{40}{23}}+ C$
$= - \frac{13}{2x^{2}} - 26\ln(|x|) + \frac{23}{4}x^{\frac{40}{23}}+ C$


##### c) Integrate $\int (10 \sin(3x) + 8 \tan( \frac{x}{2} ))$
$\int (10 \sin(3x) + 8 \tan( \frac{x}{2} ))$
-> $- \frac{1}{3}\times10 \cos(3x) + 8\times -\frac{1}{\frac{1}{2}} \ln \left(\cos \left( \frac{x}{2} \right) \right)+ C$
-> $- \frac{10}{3} \cos(3x) + 8\times - 2 \ln \left(\cos \left( \frac{x}{2} \right) \right)+ C$
$= - \frac{10}{3} \cos(3x) -16 \ln\left(\cos \left( \frac{x}{2} \right) \right)+ C$


##### d) Integrate $\int ( 6e^{4x} - 27e^{-9x} )$
$\int ( 6e^{4x} - 27e^{-9x} ) + C$
-> $\frac{6}{4}e^{4x} - \frac{27}{-9}e^{-9x} + C$
$= \frac{3}{2}e^{4x} + 3e^{-9x} + C$


### 2) Find the original function $f(x)$ given $f'(x) = 8x^{3} - 38x^{2} + 56$ and $f(-2) = 1$
**Finding the non-definite integral**
$\int(8x^{3} - 38x^{2} + 56) + C$
-> $\frac{8}{4}x^{4} - \frac{38}{3}x^{3} + 56x + C$
-> $2x^{4} - \frac{38}{3}x^{3} + 56x + C$

**Calculating using $f(-2) = 1$**
$y = 2x^{4} - \frac{38}{3}x^{3} + 56x + C$
-> $1 = 2(-2)^{4} - \frac{38}{3}(-2)^{3} + 56(-2) + C$
-> $1 = 2(16) - \frac{38}{3}(-8) - 112 + C$
-> $1 = 32 + \frac{304}{3} - 112 + C$
-> $C = 1 - 32 - \frac{304}{3} + 112$
-> $C = 81 - \frac{304}{3}$
$C = - \frac{61}{3}$

**Answer**
$f(x) = 2x^{4} - \frac{38}{3}x^{3} + 56x - \frac{61}{3}$ given $y=1$ and $x=-2$


### 3) Find the original function $f(x)$ given $f'(x) = 8\sin(3x) + 12\cos(13x)$ and $f(-\pi) = 2$
**Finding the non-definite integral**
$\int (8\sin(3x) + 12\cos(13x)) + C$
-> $- \frac{1}{3}\times 8 \cos(3x) + \frac{1}{13}\times12 \sin(13x) + C$
-> $- \frac{8}{3} \cos(3x) + \frac{12}{13} \sin(13x) + C$

**Calculating using $f(-\pi) = 2$**
$y = - \frac{8}{3} \cos(3x) + \frac{12}{13} \sin(13x) + C$
-> $2 = - \frac{8}{3} \cos(3(-\pi)) + \frac{12}{13} \sin(13(-\pi)) + C$
-> $2 = - \frac{8}{3} \cos(-3\pi)) + \frac{12}{13} \sin(-13\pi)) + C$
-> $2 = - \frac{8}{3} \times -1 + \frac{12}{13} \times 0 + C$
-> $2 = \frac{8}{3} + C$
-> $C = 2 - \frac{8}{3}$
-> $C = \frac{6}{3} - \frac{8}{3}$
$C = - \frac{2}{3}$

**Answer**
$f(x) - \frac{8}{3} \cos(3x) + \frac{12}{13} \sin(13x) - \frac{2}{3}$ given $x = -\pi$ and $y=2$

### 4) Find the original function $f(x)$ given $f'(x) = \frac{23}{x}$ and $f(e) = 3$
**Finding the non-definite integral**
$\int\left( \frac{23}{x} \right)+ C$
-> $23\ln( |x| ) + C$

**Calculating using $f(e) = 3$**
%% [[Log Laws - Log base of base]] %%
$y = 23\ln( |x| ) + C$
-> $3 = 23\ln( |e| ) + C$
	-> We apply the $\log_{e}(e) = 1$ rule
-> $3 = 23\times1 + C$
-> $3 - 23 = C$
$C = -20$

**Answer**
$f(x) = 23\ln( |x| ) - 20$ given $x=e$ and $y=3$
