---
tags:
  - portfolio/worksheets/7/2C
received-week: 8
due-week: 10
due-date: 2024-05-03T00:00:00
finished: true
submitted: true
todo: 
topics:
---
# Task 1: Differentiation
### 1) Find the derivative of the following functions
##### <mark style="background: #FFB8EBA6;">a)</mark> $y= \frac{ 4x^{5} - 7x^{2} + 3x - 8 }{ x - 3 }$
%% 
- [[The Derivative]]
- [[Derivatives of fractions]]
- [[Quotient Rule]] 
%%
We want to use the quotient rule here, $f'(x) = \frac{vu' - uv'}{v^{2}}$
$u = 4x^{5} - 7x^{2} + 3x - 8$
-> $5\times4x^{5-1} + 2\times-7x^{2-1} + 3\times1x^{1-1} \cancel{-8}$
$u' = 20x^{4} -14x + 3$

$v = x-3$
-> $x^{1-1} \cancel{-3}$
$v' = 1$

**Expanding $vu' - uv'$**
$\frac{ (x-3)(20x^{4} - 14x + 3) - (4x^{5} - 7x^{2} + 3x  - 8)(1)  }{ (x-3)^{2} }$
-> $(x-3)(20x^{4} - 14x + 3)$
	-> $20x^{5}-14x^{2}+3x -60x^{4} +42x - 9$
-> $- (4x^{5} - 7x^{2} + 3x  - 8)$
	-> $-4x^{5} + 7x^{2} -3x + 8$

$20x^{5}-14x^{2}+3x -60x^{4} +42x - 9 -4x^{5} + 7x^{2} -3x + 8$
-> $20x^{5}-14x^{2} \cancel{+3x} -60x^{4} +42x - 9 \cancel{-4x^{5}} \cancel{+ 7x^{2}} \cancel{-3x} \cancel{+ 8}$
-> $16x^{5} - 60x^{4} - 7x^{2} + 42x - 1$

$(x-3)^{2}$ is already simplified, so:

**Solution: Derivative of $y$**
$y' = \frac{16x^{5} - 60x^{4} - 7x^{2} + 42x - 1}{(x-3)^{2}}$


##### <mark style="background: #FF5582A6;">b)</mark> $y = \ln(3x^{3} - x^{2} + 2)$
%% [[Derivatives of logs and e]] %%

$u = 3x^{3} - x^{2} + 2$
-> $3\times3x^{3-1} - 1\times2x^{2-1} \cancel{+2}$
$u' = 9x^{2} - 2x$

$v' = \frac{1}{u}$

$u' \times v'$
-> $y' = \frac{9x^{2} - 2x}{ 3x^{3}- x^{2} + 2 }$


##### <mark style="background: #FFB86CA6;">c)</mark> $y = e^{3x} \cos(2x - 5)$
%% 
- [[Derivatives of trigonometric functions]] 
- [[Product Rule]] 
%%
This problem employs the product rule, $u v' + vu'$.

%% [[Derivatives of logs and e]] %%
We use the $f'(x) = ke^{kx}$ to find the $e$ derivative 
$u = e^{3x}$
$u' = 3e^{3x}$

%% [[Derivatives of trigonometric functions]] %%
We use $f'(x) = -k \sin(kx)$ 
$v = \cos(2x-5)$
$v' = -2 \sin(2x-5)$

Finally, add all the variables together..
$u v' + vu'$
$e^{3x} \times -2\sin(2x-5) + \cos(2x-5) \times 3e^{3x}$
-> $-2e^{3x}\sin(2x-5) + 3e^{3x}\cos(2x-5)$

to get the derivative of $y$
$y' = e^{3x}(-2\sin(2x-5) + 3\cos(2x-5))$

### 2) The distance of a particle from a point, $O$, at time $t$ seconds is given by $s = 2t^{3} + 27t^{2} + 105t - 50$ metres for $t \geq 0$

$s$ is the displacement in metres, $t$ is time in seconds

##### <mark style="background: #FF5582A6;">a) Find the velocity and acceleration at time</mark> $t$
**Velocity $(s')$**, the rate of change of the displacement
$s = 2t^{3} + 27t^{2} + 105t - 50$
-> $2\times3t^{3-1} + 27\times2t^{2-1} + 105t^{1-1} \cancel{-50}$
-> $6t^{2} + 54t^{1} + 105t^{0}$
$v = 6t^{2} + 54t + 105$

**Acceleration $(s'')$**, the rate of change of the velocity
$6t^{2} + 54t + 105$
-> $2\times6t^{2-1} + 54\times1t^{1-1} \cancel{105}$
$a = 12t + 54$

##### <mark style="background: #FF5582A6;">b) Find the time(s) when the particle has a velocity of zero. Give the displacement & acceleration at these times</mark>.
Plan: Set velocity to zero, find $t$, then plug $t$ into the acceleration and displacement equations

**Finding the times ($t_{1}$ and $t_{2}$)**
$v = 6t^{2} + 54t + 105$
-> $0 = 6t^{2} + 54t + 105$
-> $t = \frac{ -(54) \pm \sqrt{ (54)^{2} - 4(6)(105) } }{ 2(6) }$
-> $t = \frac{ -54 \pm \sqrt{ 2916 - 2520 } }{ 12 }$
-> $t = \frac{ -54 \pm \sqrt{ 396 } }{ 12 }$
$t_{1}^{+} = -2.842$s
$t_{2}^{-} = -6.158$s
The times are negative so next equations don't exactly make sense as time cannot traditionally be negative, but they are correct.

**Acceleration at velocity of $0$ $\ce{m/s^{2}}$**
$a = 12t_{1} + 54$
-> $a_{1} = 12(-2.842) + 54$
$a_{1} = 19.8997$ $\ce{m/s^{2}}$

$a = 12t_{2} + 54$
-> $a_{2} = 12(-6.158) + 54$
$a_{2} = -19.8997$ $\ce{m/s^{2}}$

Interestingly but perhaps not coincidentally, the acceleration function reverses the quadratic equation division and $-b$ term.


**Finding the displacement at a velocity of 0$\ce{m/s^{2}}$**
$s = 2t_{1}^{3} + 27t_{1}^{2} + 105t_{1} - 50$
-> $s = 2(-2.842)^{3} + 27(-2.842)^{2} + 105(-2.842) - 50$
$-176.2414$ metres


$s = 2t_{2}^{3} + 27t_{2}^{2} + 105t_{2} - 50$
-> $s = 2(-6.158)^{3} + 27(-6.158)^{2} + 105(-6.158) - 50$
$s = -139.7586$ metres


**Zero seconds elapsed**
$s = 2t^{3} + 27t^{2} + 105t - 50$
-> $s = 2(0)^{3} + 27(0)^{2} + 105(0) - 50$
$s = -50$ metres


This implies that $-2.8$ and $-6.2$ seconds in the past, the object was displaced negative distances. Granted, this is from the point of observation. At $-2.8$ seconds, relatively it would have been at $0$m displaced, we're simply saying that $0$ seconds elapsed is the present, even though at zero seconds, we are $-50$ metres behind. This question broaches subjects uncomfortable to the fettered mind.

### <mark style="background: #FFF3A3A6;">3) Find the stationary points of the function</mark> $y = x^{3} + \frac{11}{2}x^{2} - 4x + 31$
- Use a sign diagram to classify each of the stationary points.
- Use the second derivative test to classify each of the stationary points. 
- Explain which method you prefer and why.
$y = x^{3} + \frac{11}{2}x^{2} - 4x + 31$
-> $3x^{3-1} + 2\frac{11}{2}x^{2-1} - 4x^{1-1} \cancel{+31}$
$y' = 3x^{2} + 11x - 4$

Finding $y''$
-> $3x^{2} + 11x - 4$
-> $2\times3x^{2-1} + 11x^{1-1} \cancel{-4}$
-> $6x^{1} + 11x^{0}$
$y'' = 6x + 11$


##### Finding the stationary points ($y''$ method)
$(x_{1},y_{1}): (\frac{1}{3}, 30.315)$
$(x_{2},y_{2}): (-4, 71)$

###### Working out
$0 = 3x^{2} + 11x - 4$
-> $x= \frac{ -(11) \pm \sqrt{ (11)^{2} - 4(3)(-4) } }{ 2(3) }$
-> $x= \frac{ -11 \pm \sqrt{ 121 + 48 } }{ 6 }$
	-> $121 + 48 \to \sqrt{169}$
-> $x = \frac{-11 \pm 13}{6}$
$x_{1}^{+} = \frac{2}{6} = \frac{1}{3}$
$x^{-}_{2} = - \frac{24}{6} = - \frac{4}{1} = -4$

$y_{1} = x^{3} + \frac{11}{2}x^{2} - 4x + 31$
-> $\frac{1}{3}^{3} + \frac{11}{2}(\frac{1}{3})^{2} - 4(\frac{1}{3}) + 31$
-> $\frac{1}{27} + \frac{11}{2} \frac{1}{9} - \frac{4}{3} + 31$
-> $\frac{1}{27} + \frac{11}{18} - \frac{4}{3} + 31$
-> $\frac{2}{54} + \frac{33}{54} - \frac{72}{54} + 31$
-> $-\frac{37}{54} + \frac{1674}{54}$
-> $\frac{1637}{54}$
$= 30.315$

$y_{2} = x^{3} + \frac{11}{2}x^{2} - 4x + 31$
-> $-4^{3} + \frac{11}{2}(-4)^{2} - 4(-4) + 31$
-> $-64 + \frac{176}{2} + 16 + 31$
-> $88 -17$
$y_{2} = 71$






##### Classifying the points
Points:
- $(\frac{1}{3}, 30.315)$
- $(-4, 71)$

###### Derivative of the derivative test
$y'' = 6x + 11$
-> $6\left(\frac{1}{3}\right)+ 11$
-> $2 + 11$
-> $13$
As $13>0$, point $(\frac{1}{3}, 30.315)$ is a local minimum

$y'' = 6x + 11$
-> $6(-4) + 11$
-> $-24 + 11$
-> $-13$
As $-13<0$, point $(-4, 71)$ is a local maximum

###### Sign test
$y' = 3x^{2} + 11x - 4$

$3( \frac{1}{3} \pm \frac{1}{3} )^{2} + 11( \frac{1}{3} \pm \frac{1}{3} ) - 4$
-> $x=0 \rightarrow 4.6\dot{6}$
-> $x= \frac{2}{3} \rightarrow -4$

$y' = 3( -4 \pm 1 ) ^{2} + 11( -4 \pm 1 ) - 4$
-> $x = -5 \to 16$
-> $x = -3 \to -10$

| Points                  | $<x$ | $x=0$ | $x>$ | Answer        |
| ----------------------- | ---- | ----- | ---- | ------------- |
| $(\frac{1}{3}, 30.315)$ | $-$  | $0$   | $+$  | Local minimum |
| $(-4,71)$               | $+$  | $0$   | $-$  | Local maximum |
It is a local minimum as the left side is descending downwards $(-)$ into the stationary point ($0$) which then it ascends $(+)$. Same but reverse for the local maximum: It ascends ($+$) until the point $(0)$ then it descends $(-)$.


##### Preferred method explanation
I prefer the $y''$, double derivative method. The sign method feels untrustworthy and seemingly reliant on trial-and-error. I got the 'wrong answers' multiple times using the sign test even though I was told and had seen multiple resources saying that you can use *any* value below/above $x$. From my trials, this is not true, and unless otherwise learnt, I will not be using the sign test due to it's unpredictability. 
In retrospect after writing this, I believe the sign test will work every time if the function is not a polynomial past quadratics. More than one stationary point means the test will always give a wrong answer.
The $y''$ method works no matter the amount of points and since it seems to usually be fairly condensed by the time you derive the original function so many times, it is trivial to do so.