
$\frac{x^{2}-x^{-1}}{x^{4}-x^{-2}}$
-> $x^{-1} = \frac{1}{x^{1}}$
-> $x^{-2} = \frac{1}{x^{2}}$

-> $\frac{x^{2}}{x^{2}}\times \frac{x^{2}-x^{-1}}{x^{4}-x^{-2}}$
-> $\frac{x^{2}(x^{2}-x^{-1})}{x^{2}(x^{4}-x^{-2})}$
-> $\frac{x^{4} + x^{1}}{x^{6}-x^{0}}$
-> $\frac{x^{4} + x}{x^{6}-1}$
 
$\frac{ (x^{\frac{3}{2}} - 1) (x^{\frac{3}{2}} + 1) }{x^{5}-x^{-1}}$
-> Expand brackets
	-> $x^{\frac{3}{2}} \times x^{\frac{3}{2}} = x^{\frac{6}{2}}= x^{3}$
	-> $x^{\frac{3}{2}} \times 1 = x^{\frac{3}{2}}$
	-> $x^{\frac{3}{2}} \times -1 = -x^{\frac{3}{2}}$ 
	-> $-1 \times 1 = -1$
-> $\frac{ x^{3} - 1 }{ x^{5} - x^{-1} }$
We want to make the exponents positive ($\geq 0$). Following exponent law rule 1, multiplication adds, so we target the $x^{-1}$ by adding $x^{1}$ to it via multiplication.
$\frac{x^{1}}{x^{1}} \times \frac{ x^{3}-1 }{ x^{5} - x^{-1}}$
-> $\frac{ x(x^{3}-1) }{ x(x^{5} - x^{-1})}$
-> $\frac{ x^{3+1}-x }{ x^{5+1} - x^{-1+1}}$
-> $\frac{ x^{4} - x }{ x^{6} - x^{0}}$
-> $\frac{ x^{4} - x }{ x^{6} - 1}$



[[Week 5 - Workshop.pdf#page=15]]


$log_{3}(12) - log_{3}(4)$
-> $log_{3}\left(\frac{12}{4}\right)= log_{3}(3) = 1$

$3log_{5}2 - log_{5}(16) + 2log_{5}(10)$
-> $log_{5}(2^{3}=8) - log_{5}(16) = log_{5}\left(\frac{8}{16}\right)= log_{5}(0.5)$
-> + $log_{5}(10^{2})= log_{5}(100)$
-> $log_{5}(0.5) + log_{5}(100) = log_{5}(100\times0.5) = log_{5}(50)$

$log_{4}(16) + log_{4}(1)$
-> $log_{4}(16\times1) = log_{4}(16)$

$log_{2}(3x) + 2log_{2}(x) - log_{2}(x)$

