---
tags:
  - portfolio/worksheets/4/2C
received-week: 4
due-week: 7
due-date: 2024-04-15T00:00:00
finished: true
submitted: true
todo: "-"
topics:
  - "[[Polynomial functions]]"
  - "[[Logarithms (log)]]"
---
# Task 1: Quadratics
## <mark style="background: #BBFABBA6;">1.1)</mark> State the number of real solutions + explain using discriminant

**Discriminant equation**
$b^{2} - 4ac$

#### <mark style="background: #BBFABBA6;">a)</mark> $-x^{2} - 3x - 10 = 0$
**Discriminant** 
-> $-3^{2} - 4(-1)(-10)$
-> $9 - 4 \times 10$
-> $= -31$

There are no real solutions as the discriminant is negative, $\sqrt{-31}$ being a complex number.

#### <mark style="background: #BBFABBA6;">b)</mark> $5x^{2} - 150 = 0$
**Discriminant**
-> $0^{2} - 4(5)(-150)$
-> $-20 \times -150$
-> $-2\cancel{0} \times -15\cancel{0}$
-> $30$

There are two real solutions as the discriminant is a positive, non-zero value.

#### <mark style="background: #BBFABBA6;">c)</mark> $25x^{2} - 20x + 4 = 0$
**Discriminant**
-> $-20^{2} - 4(25)(4)$
-> $400 - 100 \times 4$
-> $400 - 400 = 0$

The discriminant is zero, meaning there is only one unique solution.


## <mark style="background: #FFB8EBA6;">1.2) </mark>Complete the square and identify stationary points
##### <mark style="background: #FFB8EBA6;">a)</mark> $y=x^{2} - 6x + 17$
**Find $\frac{b^{2}}{4}$**
-> $\frac{-6^{2}}{4} = \frac{36}{4} = 9$

**Add $\frac{b^{2}}{4}$ to the equation**
-> $y = x^{2} -6x + 9 + 17 - 9$
-> $y = x^{2} -6x + 9 + 8$

**Form a perfect square**
-> $y = (x^{2} -6x + 9) + 8$
	-> $-3\times-3 = 9$ and $-3 + -3 = -6$
-> $y = (x - 3)^{2} + 8$

**Extract the vertex**
$y = (x - 3)^{2} + 8$
-> $x$ is translated by $-3$, so $x=3$
-> $y = 8$

**Vertex = $(3,8)$**

*Verification*
$x = \frac{-b}{2a} \rightarrow \frac{--6}{2(1)} = \frac{6}{2} = 3$
$y = 3^{2} - 6(3) + 17$
-> $9 - 18 + 17$
-> $y=-9 + 17 = 8$
$(3,8)$


##### <mark style="background: #FFB8EBA6;">b)</mark> $y=3x^{2} - 12x + 6$
**Divide by $a$**
$y=3x^{2} - 12x + 6$
-> $y=\frac{3x^{2}}{2} - \frac{12x}{2} + \frac{6}{2}$
-> $3(x^{2} - 4x + 2)$

**Find $\frac{b^{2}}{4}$**
$3(x^{2} - 4x + 2)$
-> $\frac{-4^{2}}{4} = \frac{16}{4} = 4$

**Add $\frac{b^{2}}{4}$ to the equation**
$3(x^{2} - 4x + 2)$
-> $3(x^{2} - 4x + 4 + 2 - 4)$
-> $3(x^{2} - 4x + 4 -2 )$


**Form a perfect square**
$3(x^{2} - 4x + 4 -2 )$
-> $3((x^{2} - 4x + 4) -2 )$
	-> $-2 \times -2 =4$, added they $=-4$. $-2$ is therefore the factor.
-> $3((x - 2)^{2} -2 )$

**Extract the vertex**
$y=3((x - 2)^{2} -2 )$
-> $x$ is translated by $-2$, so $x = 2$
-> $y = 3(-2) = -6$

**Vertex = $(2, -6)$**


*Verification*
$x = \frac{-b}{2a} = \frac{--12}{2(3)} = \frac{12}{6} = 2$
-> $x=2$

$y=3x^{2} - 12x + 6$
-> $3(2^{2}) - 12(2) + 6$
-> $3(4) - 24 + 6$
-> $12 - 24 + 6$
-> $-12 + 6$
-> $y = -6$

$= (2, -6) = \ce{vertex}$


## <mark style="background: #FF5582A6;">1.3)</mark> Find the solutions for $4x^{2} - 3x = 10$

$4x^{2} - 3x = 10$
-> $4x^{2} - 3x - 10 = 0$
-> $x= \frac{ -(-3) \pm \sqrt{ (-3)^{2} - 4(4)(-10) } }{ 2(4) }$
-> $x= \frac{ 3 \pm \sqrt{ 9 - -160 } }{ 8 }$
-> $x= \frac{ 3 \pm \sqrt{ 169 } }{ 8 }$
-> $x= \frac{ 3 \pm 13 }{ 8 }$

$x^{+} = \frac{3+13}{8} = \frac{16}{8} = 2$
$x^{-} = \frac{3-13}{8} = \frac{-10}{8} = -\frac{5}{4}$





# Task 2: Logarithms and Exponentials
## <mark style="background: #FFB8EBA6;">2.1)</mark> Solve for $x$ using log and exponent rules
%%[[Logarithms (log)]] %%
##### <mark style="background: #FFB8EBA6;">a)</mark> $2y = 10 + e^{3x-4}$
-> $2y - 10 = e^{3x-4}$
-> $ln(2y - 10) = ln(e^{3x-4})$
-> $ln(2y - 10) = 3x-4$
-> $ln(2y - 10) + 4 = 3x$
-> $\frac{ln(2y - 10) + 4}{3} = x$
$x=\frac{ln(2y - 10) + 4}{3}$


##### <mark style="background: #FFB8EBA6;">b)</mark> $\ce{ln}(2x-3) + \ce{ln}(x+2) = \ce{ln}(9x-24)$
Apply $log_{a}(a)=1$ to both sides of the equation 
%%[[Log Laws - Log base of base]]%%
-> $e^{ln(2x-3)} + e^{ln(x+2)} = e^{ln(9x-24)}$
-> $2x-3 + x + 2 = 9x-24$
-> $3x -1 = 9x-24$
-> $-1 + 24 = 9x-3x$
-> $23 = 6x$
$x = \frac{23}{6}$

## <mark style="background: #FF5582A6;">2.2)</mark> Expand and simplify $(2e^{2x} - e^{-2x} )^{2}$
$a^{2} - 2ab + b^{2}$
-> $(2e^{2x})^{2} - 2(2e^{2x})(-e^{-2x}) + (-e^{-2x})^{2}$
- $2^{2}e^{4x} = 4e^{4x}$
- $-2(2e^{2x}) = -4e^{2x}$
- $-4e^{2x} \times e^{-2x} = -4e^{2x  + -2x} = 4e^0 = -4$
	- $(-e^{-2x})(-e^{-2x}) = e^{-2x+-2x} = e^{-4x}$ 
$4e^{4x} + e^{-4x} - 4$


**Verification**
$4e^{4x} + e^{-4x} - 4$
-> $4e^{4(0)} + e^{-4(0)} -4$
-> $4*1 + 1 -4$
-> $4 + 1 - 4 = 1$

$(2e^{2x} - e^{-2x} )^{2}$
-> $2e^{2(0)} - e^{-2(0)}$
-> $(2 - 1)^{2} = (1)^{2}$
-> $1$


## <mark style="background: #BBFABBA6;">2.3)</mark> Simply $2ln(xy) + ln(x) - ln(x^{3}y^{2})$
$2ln(xy) + ln(x) - ln(x^{3}y^{2})$

**Prepare $2ln(xy)$ for addition using the expansion log law**
%% [[Log Laws - Log(m raised to n)]] %%
$log_{a}(m^{n})=(n)log_{a}(m)$
-> $2ln(xy) \rightarrow ln((xy)^{2})$

**Add them together using the addition log law** 
%% [[Log Laws - Addition]]%%
$log_{a}(m)+log_{a}(n)=log_{a}(mn)$
-> $ln((xy)^{2} \times x)$
-> $x^{2}y^{2} \times x$
-> $x^{3}y^{2}$
$ln(x^{3}y^{2})$

**Subtraction**
$log_{a}(m)-log_{a}(n)=log_{a}(\frac{m}{n})$
-> $ln(x^{3}y^{2}) - ln (x^{3}y^{2}) = ln(\frac{x^{3}y^{2}}{x^{3}y^{2}})$
-> $ln(\frac{x^{3}y^{2}}{x^{3}y^{2}})$
-> $ln(\frac{x^{0}y^{0}}{x^{0}y^{0}})$
-> $ln( \frac{1\times1}{1\times1})$
##### $ln(1) = 0$


# Task 3: Trigonometry
![[4.2C - Figure 1 triangle for Task 3.png|150]]
## <mark style="background: #D2B3FFA6;">3.1)</mark> Find $b$'s length, $\theta$, and $\phi$. Angles must be in radians and to 4 decimal places.
$b = 4\sqrt[]{2}$
$\theta = 0.8911$ radians
$\phi = 0.6797$ radians 

$b=\sqrt{ c^{2} - a^{2} }$
-> $b=\sqrt{ 9^{2} - 7^{2} }$
-> $b=\sqrt{ 81 - 49 }$
-> $b = \sqrt[]{32}$
	-> $32 = 2 * 16$
-> $b = \sqrt[]{16} \sqrt[]{2}$
$b = 4\sqrt[]{2}$

$\theta = \arctan\left(\frac{7}{4\sqrt[]{2}}\right)= 0.8911$ radians
- $\theta = \arccos\left(\frac{4\sqrt{2}}{9}\right)= 0.8911$ radians
- $\theta = \arcsin(\frac{7}{9}) = 0.8911$ radians

$360\degree = 2\pi$ radians, so $180\degree = \pi$ radians and $90\degree = \frac{\pi}{2}$ radians
According to the triangle law, a triangle's sum of angles is $180\degree$.
-> $180\degree - 51.06\degree - 90\degree = 38.94\degree$
$\pi - 0.8911 - \frac{\pi}{2} = 0.6797$ radians

## <mark style="background: #FFB86CA6;">3.2)</mark> If $\cos(\theta) = \frac{-\sqrt{3}}{2}$ and $\sin(\theta)= \frac{-1}{2}$, which quadrant does angle $\theta$ belong to?
A negative value divided by a positive still leads to a negative value, so $\cos = -x$ and $\sin=-y$. Following AS*T*C, Angle $\theta$ must therefore belong to the third quadrant as $\tan$ would be positive when both $\sin$ and $\cos$ are negative.

## <mark style="background: #FFB8EBA6;">3.3)</mark> Sketch $y=2\cos(x)$ for $x \in [0,2\pi]$. What is the range and $x/y$-intercepts?
The domain is $0 \leq x \leq 2\pi$.
The range of $\cos$ is $-1 \leq x \leq 1$, but as it is multiplied by $2\times$, the range of this function is $-2 \leq x \leq 2$

**y-intercept**
$y=2\cos(x)$
-> $y=2\cos(0)$
-> $y = 2\times1$
$y = 2$

**x-intercept**
$y=2\cos(x)$
-> $0=2\cos(x)$
-> $\frac{0}{2} = \cos(x)$
-> $\arccos(0) = x$
$x = 1.5708 = \frac{\pi}{2}$
It took $x=\frac{\pi}{2}$ to do half of a full dip, reaching $y=0$. $\cos$ waves rise back up, so it must take $\frac{\pi}{2}$ for the first half of the down dip to reach $y=0$, $\frac{\pi}{2}$ for the second half of the dip ($y=-1$), and on the upwards rise, another $\frac{\pi}{2}$, totalling $3 \frac{\pi}{2} = \frac{3\pi}{2}$ where $y=0$ again. 
At this point, it will have reached another $x$ intercept. So, the $x$ intercepts are $\frac{\pi}{2}$ and $\frac{3\pi}{2}$.
A general formula found with the help of the internet is $\frac{\pi}{2} + 2\pi n$.


<mark style="background: #FF5582A6;"><b>Graph</b></mark>
![[4.2C - Task 3 Q3.3 graph.jpg|400]]