**Links**
- [[Quadratics#Turning point form]] 
- [[Quadratic formula]] 
- [[4.1P]] 

https://www.youtube.com/watch?v=7xE5pj9-n1Q

If the coefficient of $x^{2}$ is not 1, then divide by this coefficient
	e.g. $2x^{2} - 4x + 8 \rightarrow 2(x^{2} -2x + 2)$

Identify the coefficient $b$ of the $x$ term
	$x^{2} - 2x + 2$ has $b=-2$

Add $\frac{b^{2}}{4} - \frac{b^{2}}{4}$ to the quadratic
	$2(x^{2} - 2x + 2 + (\frac{-2^{2}}{4}) - (\frac{2^{2}}{4}))$
	= $2(x^{2} - 2x + 2 + 1 - 1)$
	$=2(x^{2} - 2x + 2)$
	$=2((x-1)^{2} + 1)$	

Finally, 
$y = 2(x-1)^{2} + 2$


$x^{2} - 4x + 8$
$x^{2} - 4x + 4 + 8 - 4$
$y=(x-2)^{2} + 4$


#### $x^{2} - 6x  + 27$
-> $\frac{-6^{2}}{4} = \frac{36}{4} = 9$
-> $x^{2} - 6x + 9 + 27 - 9$
	-> Factors of 9:
		(1,9)=10
		(3,3)=6
-> $(x-3)^{2} + 18$

**Using the $(x-3)^{2} + 18$, solve $x^{2}-6x+27 = 99$****
-> $99 = (x-3)^{2} + 18$
-> $81 = (x-3)^{2}$
-> $\pm \sqrt{81} = x-3$
-> $\pm 9 + 3 = x$
-> $x = 12$ or $x=-6$ 
