**Links**
- [[Quadratics]] 
- [[Quadratic formula]] 
- [[Factorising and expanding]] 

Generate practice problems here: https://www.wolframalpha.com/problem-generator/quiz/?category=Algebra&topic=FactorQuadraticPolynomial
 
### Examples
$x^{2} - 36 = 0$
-> $(x-6)(x+6)=0$


$x^{2} -10x + 24$
-> 24 factors: (1,24)=25, **(6,4)=10**, (3,8)=11
-> $(x-4)(x-6)$


$x^{2} - 11x + 28$
-> 28's factors: 
	- (1,28)=29
	- (2,14)=16
	**- (4,7)=11**
-> $(x-4)(x-7)$

# $-6w^{2} - 32w - 42$
$-6w^{2} - 32w - 42$
-> $-2(3w^{2} +16w + 21)$
Find factors of $a * c = 3 * 21 \rightarrow 63$ that sum to $16$:
- $21 * 3$ adds to $24$
- $7 * 9$ adds to $16$, so we choose these factors
$3w^{2} +16w + 21$
-> $3w^{2} + 7w + 9w + 21$
-> $(3w^{2} + 7w) + (9w + 21)$
	$3w^{2} + 7w$
		$w(3w+7)$
	$9w+21$
		$3w(3w+7)$
$3(3w + 7) + w(3w+7)$

$(3w+7)$ are common factors so we can factor it out.
Furthermore, the outer $3$ and $w$ combine to form ($3+w$)
-> $3() + w()$
	-> $(3 + w)$
$(3+w)(3w+7)+(3w+7)$
-> $() + \cancel{()}$
	-> $(3w+7)$
-> $(3w + 7)(3+w)$
Finally, don't forget the $-2$ we started with!
**Final simplified equation:** $-2((w+3)(3w+7))$


# $10w^{2} + 15w - 70$
$10w^{2} + 15w - 70$
Find the lowest common factor between $a,b,c$
-> $5(2w^{2}+3w-14)$
Find the factors of $ac$ that sum to $b$
-> $ac = 2*-14 = -28$, $b=3$
	-> $2 * 14$, additions could be $[2+-14=-12], [-2+14=12], \& [2 + 14 = 16]$
	-> $4 * 7$, additions could be $[4+7=11], [-4+7=3], \& [4+-7=-3]$
		-> The factors are therefore $-4$ and $7$ as they add to $b$
Split the equation into it's factors
-> $2w^{2}+3w-14$
-> $2w^{2} - 4w + 7w -14$
-> $(2w^{2} - 4w) + (7w -14)$
Simplify these
-> $2w(w-2) + 7(w-2)$
Factor $2w$ with $7$ and factor $(w-2)$
-> $(2w + 7)(w-2)$
Finally, re-add the initial multiplication factor
$5(2w + 7)(w-2)$


# $-m^{2} + m  + 30$
$-m^{2} + m  + 30$
**Find the lowest common factor between $a,b,c$**
-> $-1(m^{2} - m  - 30)$
**Find the factors of $ac$ that sum to $b$**
-> $ac = 1*-30 = -30$, $b=-1$
	-> $1 * 30: [1+30=31],[-1+30=29],[1+-30=-29]$
	-> $3*10: [3+10=13], [-3+10=7], [3-10=-7]$
	-> $6*5: [6+5=11], [-6+5=-1], [6-5=1]$
		-> We pick factors $6$ and $-5$
**Split the equation into it's factors**
$m^{2} - m  - 30$
-> $m^{2} + 6m - 5m  - 30$
$(m^{2} + 6m) - (5m  - 30)$

**Simplify these**
-> $m(m + 6) + -5(m + 6)$

**Factor $m, -5$ and $(m+6)$**
-> $(m - 5)(m+6)$

**Re-add the initial $a$ value**
-> $-1(m - 5)(m+6)$


# $12x^{2} + 49x + 49$
$12x^{2} + 49x + 49$
$a$ can't be factored out in the example, so unfortunately, we need to find factors of  $ac = 12 * 49 = 588$ that sum to $a+c,b=49$
By sheer coincidence, $5+8+8 = 21$, $\frac{588}{21} = 28$, so the two factors are $28$ and $21$.

-> $12x^{2} + 21x + 28x + 49$
-> $3x(4x + 7) + 7(4x + 7)$
$(x+7)(4x+7)$
