---
tags:
  - portfolio/worksheets/8/3HD
received-week: 9
due-week: 10
due-date: 2024-05-10T00:00:00
finished: true
submitted: true
todo: 
topics:
  - "[[The Derivative]]"
---
I apologise for the somewhat inconsistent formatting, I'm trying out some new things to see what I like best. The blocks with the blue bar are my favourite so far but I do like my `->` arrows. 
## (1) Find the stationary points of $y = (x^{4} − 2x^{3})e^{2x}$. Note: you must give exact values - do not approximate the stationary point values 

**Final answers:**

|                 | 1       | 2                                         | 3                                   |
| --------------- | ------- | ----------------------------------------- | ----------------------------------- |
| $x$             | $0$     | $+\sqrt{3}$                               | $-\sqrt{3}$                         |
| $y$             | $0$     | $9e^{2\sqrt{3}} - 6\sqrt{3}e^{2\sqrt{3}}$ | $\frac{9+6\sqrt{3}}{e^{2\sqrt{3}}}$ |
| $\approx(x,y)$* | $(0,0)$ | $(1.732, -44.481)$                        | $(-1.732)(0.607)$                   |
\*approximates for curiosity's sake

### Working out for (1)
**Finding $y'$**
%% [[Product Rule]] %%
$y = (x^{4} − 2x^{3})e^{2x}$
$u = x^{4} - 2x^{3}$
$u' = 4x^{3} - 6x^{2}$

$v = e^{2x}$
$v' = 2e^{2x}$

$u \times v' + v \times u'$
-> $(x^{4} - 2x^{3}) \times 2e^{2x} + e^{2x}(4x^{3} - 6x^{2})$
-> $e^{2x}(2x^{4} - 4x^{3}) + e^{2x}(4x^{3} - 6x^{2})$
-> $2e^{2x}x^{4} - 4e^{2x}x^{3} + 4e^{2x}x^{3} - 6e^{2x}x^{2}$
-> $2e^{2x}x^{4} \cancel{- 4e^{2x}x^{3} + 4e^{2x}x^{3}} - 6e^{2x}x^{2}$
-> $2e^{2x}x^{4} - 6e^{2x}x^{2}$
$y' = 2e^{2x}x^{4} - 6e^{2x}x^{2}$


#### <mark style="background: #FF5582A6;">Stationary points</mark>
$y' = 2e^{2x}x^{4} - 6e^{2x}x^{2}$
-> $0 = 2e^{2x}x^{4} - 6e^{2x}x^{2}$
-> $2e^{2x}x(x^{3} - 3x)$
-> $2e^{2x}x^{2}(x^{2} - 3)$

%% [[Difference of two squares]] %%
**Setup a difference of two squares formula, where $a^{2} - b^{2} = (a+b)(a-b)$**
$(x^{2} - 3) = x^{2} - 3 = (x)^{2} - (3)^{2}$
-> $-3 = (\sqrt{3})^{2}$
-> $(x^{2} - (\sqrt{3})^{2})$
-> $x^{2} - (\sqrt{3})^{2}$
$= (x + \sqrt{3})(x - \sqrt{3})$
Verification: -> $x^{2} + \sqrt{3}x - \sqrt{3}x - 3 = x^{2} - 3$

%% [[Zero-product property]] %%
**Apply the zero-product principle**
-> $0 = 2e^{2x}x^{2}(x^{2} - 3)(x + \sqrt{3})(x - \sqrt{3})$
- $e^{2x} = 0$ ($2 \neq 0$ so it's unneeded) or
- $x^{2} = 0$ meaning $x=0$ or
- $x - \sqrt{3} = 0$ or
- $x + \sqrt{3} = 0$ 

**Sifting for valid values**
$e^{2x} = 0$
-> $e = \sqrt[2x]{0}$
-> $\sqrt[2x]{0} = 0$
$e \neq 0$, so it is not a stationary point

$x_{1} = 0$
-> Can be true, so it's valid

$x - \sqrt{3} = 0$
-> $x_{2} = + \sqrt{3}$


$x + \sqrt{3} = 0$
-> $x_{3} = - \sqrt{3}$

So, the points on the $x$-axis are $0, \sqrt{3},$ and $-\sqrt{3}$ 


##### <mark style="background: #FF5582A6;">Finding the stationary point</mark> $y$<mark style="background: #FF5582A6;">-values</mark>
From the x-values $0, -\sqrt{3},$ and $\sqrt{3}$

**Finding $y_{1}$ from $x_{1} = 0$**
$y_{1} = ((0)^{4} − 2(0)^{3})e^{2(0)}$
-> $(0 - 0) \times 1$
$y_{1} = 0$

**Finding $y_{1}$ from $x_{2} = \sqrt{3}$**
$y_{2} = ((\sqrt{3})^{4} − 2(\sqrt{3})^{3})e^{2(\sqrt{3})}$
> $(\sqrt{3})^{4} = 9$

%% [[Roots]] %%
Applying the root rule $(\sqrt[n]{a})^{n} = a$
-> $-2(\sqrt{3})^{3}$
-> $-2(\sqrt[2]{3})^{2}\sqrt{3}$
-> $-2(3) \sqrt{3}$
$= -6\sqrt{3}$

-> $e^{2\sqrt{3}}(9 - 6\sqrt{3})$
$y_{2} = 9e^{2\sqrt{3}} - 6\sqrt{3}e^{2\sqrt{3}}$


**Finding $y_{1}$ from $x_{3} = -\sqrt{3}$**
$y_{2} = ((-\sqrt{3})^{4} − 2(-\sqrt{3})^{3})e^{2(-\sqrt{3})}$
> $(-\sqrt{3})^{4} = 9$
> $-2(-\sqrt{3})^{3} = -2(-\sqrt{3})^{2} \times -\sqrt{3}$
> $-\sqrt{3}^{2} = -3$
> $-2 \times -3 = 6$

$(9 - 6\times -\sqrt{3})e^{2(-\sqrt{3})}$
-> $(9 + 6\sqrt{3})e^{2(-\sqrt{3})}$
-> $9e^{2-\sqrt{3}} + 6\sqrt{3}e^{2(-\sqrt{3})}$

%% [[Exponent (Index) laws - Reciprocals]] %%
Apply the reciprocal index law $x^{-y} = \frac{1}{x^{y}}$
$9e^{2(-\sqrt{3})} + 6\sqrt{3}e^{2(-\sqrt{3})}$
-> $9e^{-2\sqrt{3}} + 6\sqrt{3}e^{-2\sqrt{3}}$
-> $\frac{9}{e^{2\sqrt{3}}} + \frac{6\sqrt{3}}{e^{2\sqrt{3}}}$
$y_{3} = \frac{9+6\sqrt{3}}{e^{2\sqrt{3}}}$



## (2) Draw a single sign table and an accompanying sign diagram. 
For each interval in the sign table, select a value of $x$ and show all working to obtain the sign of the gradient in that interval. 
Note: there should be no approximations in working to obtain gradient for the selected values of x. Please leave the expressions with square roots and powers of e.

#### <mark style="background: #FF5582A6;">Finding</mark> $y''$
$y' = 2e^{2x}x^{4} - 6e^{2x}x^{2}$

**Left side**
$u_{LL} = 2e^{2x}$ and $u_{LL}' = 4e^{2x}$
$v_{LR} = x^{4}$ and $v'_{LR} = 4x^{3}$

$uv' + vu' \to u_{LL}v_{LR}' + v_{LR}u_{LL}'$
$2e^{2x} \times 4x^{3} +x^{4} \times 4e^{2x}$
-> $u'_{L} = 8e^{2x}x^{3} + 4e^{2x}x^{4}$

**Right side**
$u_{RL} = 6e^{2x}$ and $u'_{RL} = 12e^{2x}$
$v_{RR} = x^{2}$ and $v'_{RR} = 2x$

$6e^{2x} \times 2x  + x^{2} \times 12e^{2x}$
-> $v'_{R} = 12e^{2x}x + 12e^{2x}x^{2}$

**Combining left and right**
$y'' = (u'_{L}) - (u'_{R})$
-> $(8e^{2x}x^{3} + 4e^{2x}x^{4}) - (12e^{2x}x + 12e^{2x}x^{2})$
-> $8e^{2x}x^{3} + 4e^{2x}x^{4} - 12e^{2x}x - 12e^{2x}x^{2}$
-> $y'' = 4e^{2x}x^{4} + 8e^{2x}x^{3} - 12e^{2x}x^{2} - 12e^{2x}x$


### <mark style="background: #FFB86CA6;">Filled out sign table</mark>
**Working out is below**

|                 | 1                   | 2                                         | 3                                        |
| --------------- | ------------------- | ----------------------------------------- | ---------------------------------------- |
| $x$             | $0$                 | $+\sqrt{3}$                               | $-\sqrt{3}$                              |
| $y$             | $0$                 | $9e^{2\sqrt{3}} - 6\sqrt{3}e^{2\sqrt{3}}$ | $\frac{9+6\sqrt{3}}{e^{2\sqrt{3}}}$      |
| $\approx(x,y)$* | $(0,0)$             | $(1.732, -44.481)$                        | $(-1.732)(0.607)$                        |
|                 |                     |                                           |                                          |
| $y''$           | $0$                 | $12\sqrt{3}e^{2\sqrt{3}}$                 | $- \frac{ 12\sqrt{3} }{ e^{2\sqrt{3}} }$ |
| $\approx y''$   | $0$, need sign test | $644.02$                                  | $-0.65$                                  |
|                 | $+,0,-$, local max  | $>0$, local min                           | $<0$, local max                          |

#### <mark style="background: #BBFABBA6;">Calculating</mark> $0$
%% [[Using derivatives to find the stationary point (vertex)]] %%
$y'' = 4e^{2x}x^{4} + 8e^{2x}x^{3} - 12e^{2x}x^{2} - 12e^{2x}x$
-> $4e^{2(0)}(0)^{4} + 8e^{2(0)}(0)^{3} - 12e^{2(0)}(0)^{2} - 12e^{2(0)}(0)$
-> $4 \times 0 + 8 \times 0 - 12 \times 0 - 12 \times 0$
$= 0$
As $0 = 0$, the sign test has to be used.

##### Sign test calculations
|                    | $x<0$ at $x=-0.1$             | $x=0$ | $x>0$ at $x=0.1$ |
| ------------------ | ----------------------------- | ----- | ---------------- |
| Exact ($=$)        | $-4e^{-2} = -\frac{4}{e^{2}}$ | $0$   | $- 12e^{2}$      |
| Approx ($\approx$) | $0.8780$                      | $0$   | $-1.6020$        |
| Results            | $+$                           | $0$   | $-$              |
The results are $+, 0, -$, that means the point must be a local maximum. 

**Calculating $+0.1$**
$y'' = 4e^{2x}x^{4} + 8e^{2x}x^{3} - 12e^{2x}x^{2} - 12e^{2x}x$
-> $4e^{2(0.1)}(0.1)^{4} + 8e^{2(0.1)}(0.1)^{3} - 12e^{2(0.1)}(0.1)^{2} - 12e^{2(0.1)}(0.1)$
-> $4e^{0.2}(0.0001) + 8e^{0.2}(0.001) - 12e^{0.2}(0.01) - 12e^{0.2}(0.1)$
-> $\frac{4}{10000}e^{\frac{1}{5}} + \frac{8}{1000}e^{\frac{1}{5}} - \frac{12}{100}e^{\frac{1}{5}} - \frac{12}{10}e^{\frac{1}{5}}$
-> $\frac{4}{10000}e^{\frac{1}{5}} + \frac{80}{10000}e^{\frac{1}{5}} - \frac{1200}{10000}e^{\frac{1}{5}} - \frac{12000}{10000}e^{\frac{1}{5}}$
$4 + 80 - 1200 - 12,000 = -13,116$
-> $- \frac{13116}{10000}e^\frac{1}{5}$
$= \frac{-3279e^\frac{1}{5}}{2500}$
$\approx -1.6020$

**Calculating $-0.1$**
$y'' = 4e^{2x}x^{4} + 8e^{2x}x^{3} - 12e^{2x}x^{2} - 12e^{2x}x$
-> $4e^{2(-0.1)}(-0.1)^{4} + 8e^{2(-0.1)}(-0.1)^{3} - 12e^{2(-0.1)}(-0.1)^{2} - 12e^{2(-0.1)}(-0.1)$
-> $4e^{-0.2}(0.0001) + 8e^{-0.2}(-0.001) - 12e^{-0.2}(0.01) - 12e^{-0.2}(-0.1)$
-> $\frac{4}{10000}e^{-\frac{1}{5}} - \frac{8}{1000}e^{-\frac{1}{5}} - \frac{12}{100}e^{-\frac{1}{5}} + \frac{12}{10}e^{-\frac{1}{5}}$
-> $\frac{4}{10000}e^{-\frac{1}{5}} - \frac{80}{1000}e^{-\frac{1}{5}} - \frac{1200}{100}e^{-\frac{1}{5}} + \frac{12000}{10}e^{-\frac{1}{5}}$
$4-80-1200+12000 = 10724$
-> $\frac{10724}{10000}e^{-\frac{1}{5}}$
-> $\frac{2681}{2500}e^{-\frac{1}{5}}$
$\approx 0.8780$


#### <mark style="background: #BBFABBA6;">Calculating</mark> $\sqrt{3}$
$y'' = 4e^{2x}x^{4} + 8e^{2x}x^{3} - 12e^{2x}x^{2} - 12e^{2x}x$
-> $4e^{2\sqrt{3}}(\sqrt{3})^{4} + 8e^{2(\sqrt{3})}(\sqrt{3})^{3} - 12e^{2\sqrt{3}}\sqrt{3}^{2} - 12e^{2\sqrt{3}}\sqrt{3}$
-> $(9\times4e^{2\sqrt{3}}) + (3\times8e^{2(\sqrt{3})}\times\sqrt{3}) - (3\times12e^{2\sqrt{3}}) - (12e^{2\sqrt{3}}\sqrt{3})$
-> $(36e^{2\sqrt{3}}) + (24\sqrt{3}e^{2(\sqrt{3})}) - (36e^{2\sqrt{3}}) - (12\sqrt{3}e^{2\sqrt{3}})$
-> $\cancel{(36e^{2\sqrt{3}})} + (24\sqrt{3}e^{2(\sqrt{3})}) - \cancel{(36e^{2\sqrt{3}})} - (12\sqrt{3}e^{2\sqrt{3}})$
-> $24\sqrt{3}e^{2\sqrt{3}} - 12\sqrt{3}e^{2\sqrt{3}}$
$= 12\sqrt{3}e^{2\sqrt{3}}$
$\approx 644.02$
$644.02>0$ so it is a local minimum

#### <mark style="background: #BBFABBA6;">Calculating</mark> $-\sqrt{3}$
$y'' = 4e^{2x}x^{4} + 8e^{2x}x^{3} - 12e^{2x}x^{2} - 12e^{2x}x$
-> $(4e^{2(-\sqrt{3})}(-\sqrt{3})^{4}) + (8e^{2(-\sqrt{3})}(-\sqrt{3})^{3}) - (12e^{2(-\sqrt{3})}(-\sqrt{3})^{2}) - (12e^{2(-\sqrt{3})}(-\sqrt{3}))$
$(4e^{2(-\sqrt{3})}(-\sqrt{3})^{4})$
-> $4e^{2(-\sqrt{3})}\times 9$
-> $36e^{2(-\sqrt{3})}$

$(8e^{2(-\sqrt{3})}(-\sqrt{3})^{3})$
-> $(8e^{2(-\sqrt{3})}(-\sqrt{3})^{2}\times(-\sqrt{3}))$
-> $8\times3 = 24$
-> $-24\sqrt{3}e^{2(-\sqrt{3})}$

$(12e^{2(-\sqrt{3})}(-\sqrt{3})^{2})$
-> $(12e^{2(-\sqrt{3})}\times 3)$
-> $(36e^{2(-\sqrt{3})})$
-> $\times -1$
-> $-36e^{2(-\sqrt{3})}$

$(12e^{2(-\sqrt{3})}(-\sqrt{3}))$
-> $-12\sqrt{3}e^{2(-\sqrt{3})}$
-> $\times -1$
-> $12\sqrt{3}e^{2(-\sqrt{3})}$


$36e^{2(-\sqrt{3})} -36e^{2(-\sqrt{3})} -24\sqrt{3}e^{2(-\sqrt{3})} + 12\sqrt{3}e^{2(-\sqrt{3})}$
-> $\cancel{36e^{2(-\sqrt{3})} -36e^{2(-\sqrt{3})}} -24\sqrt{3}e^{2(-\sqrt{3})} + 12\sqrt{3}e^{2(-\sqrt{3})}$
-> $-24\sqrt{3}e^{2(-\sqrt{3})} + 12\sqrt{3}e^{2(-\sqrt{3})}$
-> $- 12\sqrt{3}e^{2(-\sqrt{3})}$
-> $- 12\sqrt{3}e^{-2\sqrt{3}}$
$= - \frac{ 12\sqrt{3} }{ e^{2\sqrt{3}} }$
$\approx -0.65$
%% [[Exponent (Index) laws - Reciprocals]] %%
As $-0.65 < 0$, it is a local maximum