---
tags:
  - portfolio/worksheets/4/2C
received-week: 4
due-week: 7
due-date: 2024-04-15T00:00:00
finished: false
submitted: false
todo: Task 3 (trig)
topics:
  - "[[Polynomial functions]]"
  - "[[Logarithms (log)]]"
---
# Task 1: Quadratics
### 1) State the number of real solutions + explain using discriminant

**Discriminant equation**
$b^{2} - 4ac$

##### a) $-x^{2} - 3x - 10 = 0$
**Discriminant** 
**-> $-3^{2} - 4(-1)(-10)$
-> $9 - 4 \times 10$
-> $= -31$

There are no real solutions as the discriminant is negative, $\sqrt{-31}$ being a complex number.

##### b) $5x^{2} - 150 = 0$
**Discriminant**
-> $0^{2} - 4(5)(-150)$
-> $-20 \times -150$
-> $-2\cancel{0} \times -15\cancel{0}$
-> $30$

There are two real solutions as the discriminant is a positive, non-zero value.

##### c) $25x^{2} - 20x + 4 = 0$
**Discriminant**
-> $-20^{2} - 4(25)(4)$
-> $400 - 100 \times 4$
-> $400 - 400 = 0$

The discriminant is zero, meaning there is only one unique solution.


### 2) Complete the square and identify stationary points
##### a) $y=x^{2} - 6x + 17$
**Find $\frac{b^{2}}{4}$**
-> $\frac{-6^{2}}{4} = \frac{36}{4} = 9$

**Add $\frac{b^{2}}{4}$ to the equation**
-> $y = x^{2} -6x + 9 + 17 - 9$
-> $y = x^{2} -6x + 9 + 8$

**Form a perfect square**
-> $y = (x^{2} -6x + 9) + 8$
	-> $-3\times-3 = 9$ and $-3 + -3 = -6$
-> $y = (x - 3)^{2} + 8$

**Extract the vertex**
$y = (x - 3)^{2} + 8$
-> $x$ is translated by $-3$, so $x=3$
-> $y = 8$

**Vertex = $(3,8)$**

*Verification*
$x = \frac{-b}{2a} \rightarrow \frac{--6}{2(1)} = \frac{6}{2} = 3$
$y = 3^{2} - 6(3) + 17$
-> $9 - 18 + 17$
-> $y=-9 + 17 = 8$
$(3,8)$


##### b) $y=3x^{2} - 12x + 6$
**Divide by $a$**
$y=3x^{2} - 12x + 6$
-> $y=\frac{3x^{2}}{2} - \frac{12x}{2} + \frac{6}{2}$
-> $3(x^{2} - 4x + 2)$

**Find $\frac{b^{2}}{4}$**
$3(x^{2} - 4x + 2)$
-> $\frac{-4^{2}}{4} = \frac{16}{4} = 4$

**Add $\frac{b^{2}}{4}$ to the equation**
$3(x^{2} - 4x + 2)$
-> $3(x^{2} - 4x + 4 + 2 - 4)$
-> $3(x^{2} - 4x + 4 -2 )$


**Form a perfect square**
$3(x^{2} - 4x + 4 -2 )$
-> $3((x^{2} - 4x + 4) -2 )$
	-> $-2 \times -2 =4$, added they $=-4$. $-2$ is therefore the factor.
-> $3((x - 2)^{2} -2 )$

**Extract the vertex**
$y=3((x - 2)^{2} -2 )$
-> $x$ is translated by $-2$, so $x = 2$
-> $y = 3(-2) = -6$

**Vertex = $(2, -6)$**


*Verification*
$x = \frac{-b}{2a} = \frac{--12}{2(3)} = \frac{12}{6} = 2$
-> $x=2$

$y=3x^{2} - 12x + 6$
-> $3(2^{2}) - 12(2) + 6$
-> $3(4) - 24 + 6$
-> $12 - 24 + 6$
-> $-12 + 6$
-> $y = -6$

$== (2, -6)$


### 3) Find the solutions for $4x^{2} - 3x = 10$

$4x^{2} - 3x = 10$
-> $4x^{2} - 3x - 10 = 0$
-> $x= \frac{ -(-3) \pm \sqrt{ (-3)^{2} - 4(4)(-10) } }{ 2(4) }$
-> $x= \frac{ 3 \pm \sqrt{ 9 - -160 } }{ 8 }$
-> $x= \frac{ 3 \pm \sqrt{ 169 } }{ 8 }$
-> $x= \frac{ 3 \pm 13 }{ 8 }$

$x^{+} = \frac{3+13}{8} = \frac{16}{8} = 2$
$x^{-} = \frac{3-13}{8} = \frac{-10}{8} = -\frac{5}{4}$





# Task 2: Logarithms and Exponentials
### 1) Solve for $x$ using log and exponent rules
[[Logarithms (log)]] 
##### a) $2y = 10 + e^{3x-4}$
-> $2y - 10 = e^{3x-4}$
-> $ln(2y - 10) = ln(e^{3x-4})$
-> $ln(2y - 10) = 3x-4$
-> $ln(2y - 10) + 4 = 3x$
-> $\frac{ln(2y - 10) + 4}{3} = x$
$x=\frac{ln(2y - 10) + 4}{3}$


##### b) $\ce{ln}(2x-3) + \ce{ln}(x+2) = \ce{ln}(9x-24)$
Apply [[Log Laws - Log base of base]] to both sides of the equation 
-> $e^{ln(2x-3)} + e^{ln(x+2)} = e^{ln(9x-24)}$
-> $2x-3 + x + 2 = 9x-24$
-> $3x -1 = 9x-24$
-> $-1 + 24 = 9x-3x$
-> $23 = 6x$
$x = \frac{23}{6}$

### 2) Expand and simplify $(2e^{2x} - e^{-2x} )^{2}$
$a^{2} - 2ab + b^{2}$
-> $(2e^{2x})^{2} - 2(2e^{2x})(-e^{-2x}) + (-e^{-2x})^{2}$
- $2^{2}e^{4x} = 4e^{4x}$
- $-2(2e^{2x}) = -4e^{2x}$
- $-4e^{2x} \times e^{-2x} = -4e^{2x  + -2x} = 4e^0 = -4$
	- $(-e^{-2x})(-e^{-2x}) = e^{-2x+-2x} = e^{-4x}$ 
$4e^{4x} + e^{-4x} - 4$


**Verification**
$4e^{4x} + e^{-4x} - 4$
-> $4e^{4(0)} + e^{-4(0)} -4$
-> $4*1 + 1 -4$
-> $4 + 1 - 4 = 1$

$(2e^{2x} - e^{-2x} )^{2}$
-> $2e^{2(0)} - e^{-2(0)}$
-> $(2 - 1)^{2} = (1)^{2}$
-> $1$


### 3) Simply $2ln(xy) + ln(x) - ln(x^{3}y^{2})$
$2ln(xy) + ln(x) - ln(x^{3}y^{2})$

**Prepare $2ln(xy)$ for addition using [[Log Laws - Log(m raised to n)]]**
$log_{a}(m^{n})=(n)log_{a}(m)$
-> $2ln(xy) \rightarrow ln((xy)^{2})$

**Add them together using [[Log Laws - Addition]]**
$log_{a}(m)+log_{a}(n)=log_{a}(mn)$
-> $ln((xy)^{2} \times x)$
-> $x^{2}y^{2} \times x$
-> $x^{3}y^{2}$
$ln(x^{3}y^{2})$

**Subtraction**
$log_{a}(m)-log_{a}(n)=log_{a}(\frac{m}{n})$
-> $ln(x^{3}y^{2}) - ln (x^{3}y^{2}) = ln(\frac{x^{3}y^{2}}{x^{3}y^{2}})$
-> $ln(\frac{x^{3}y^{2}}{x^{3}y^{2}})$
-> $ln(\frac{x^{0}y^{0}}{x^{0}y^{0}})$
-> $ln( \frac{1\times1}{1\times1})$
##### $ln(1) = 0$


# Task 3: Trigonometry
![[4.2C - Figure 1 triangle for Task 3.png|150]]
### 1) Find $a$'s length, $\theta$, and $\phi$. Angles must be in radians.


### 2) If $cos(\theta) = \frac{-\sqrt{3}}{2}$ and $sin(\theta)= \frac{-1}{2}$, which quadrant does angle $\theta$ belong to? Two sentences max.


### 3) Sketch $y=2cos(x)$ for $x \in [0,2\pi]$. What is the range and $x/y$-intercepts?

