**Links**
- [[SIT190 - Functions, Relations, and Graphs/Weekly classes/Week 5 - Exponential and logarithmic functions/Week 5 - Notes|Week 5 - Notes]] 
- [[Week 5 - Notes - SIT191|Week 5 - Notes - SIT191]] 

$\frac{ (x^{\frac{3}{2}} - 1) (x^{\frac{3}{2}} + 1) }{x^{5}-x^{-1}}$
-> Expand brackets
	-> $x^{\frac{3}{2}} \times x^{\frac{3}{2}} = x^{\frac{6}{2}}= x^{3}$
	-> $x^{\frac{3}{2}} \times 1 = x^{\frac{3}{2}}$
	-> $x^{\frac{3}{2}} \times -1 = -x^{\frac{3}{2}}$ 
	-> $-1 \times 1 = -1$
-> $\frac{ x^{3} - 1 }{ x^{5} - x^{-1} }$
We want to make the exponents positive ($\geq 0$). Following exponent law rule 1, multiplication adds, so we target the $x^{-1}$ by adding $x^{1}$ to it via multiplication.
$\frac{x^{1}}{x^{1}} \times \frac{ x^{3}-1 }{ x^{5} - x^{-1}}$
-> $\frac{ x(x^{3}-1) }{ x(x^{5} - x^{-1})}$
-> $\frac{ x^{3+1}-x }{ x^{5+1} - x^{-1+1}}$
-> $\frac{ x^{4} - x }{ x^{6} - x^{0}}$
-> $\frac{ x^{4} - x }{ x^{6} - 1}$

